\documentclass[12pt]{article}

\usepackage{fancyhdr}
\usepackage[headheight=0.25in,margin=1in]{geometry}

\newcommand{\parens}[1]{\left( #1 \right)}

\linespread{1.25}

\begin{document}
    \pagestyle{fancy}
    \fancyhead[L]{Chapter 1}
    \fancyhead[R]{Exercises}

    \section*{Section 1.1}

    \begin{itemize}
        \item [1.)] \textbf{Problem:} Evaluate the following:
        \[
            (1 + 2i)^3, \quad
            \frac{5}{-3 + 4i}, \quad
            \parens{ \frac{2 + i}{3 - 2i} }^2, \quad
            (1 + i)^n + (1 - i)^n
        \]

        \textbf{Solutions:}

        \begin{itemize}
            \item [a.)] \( (1 + 2i)^3 = (-3 + 4i)(1 + 2i) = -11 - 2i \)
            
            \item [b.)] We have that
            \[
                \frac{5}{-3 + 4i} =
                \frac{5}{-3 + 4i} \cdot \frac{-3 - 4i}{-3 - 4i} =
                \frac{-15 - 20i}{25} =
                -\frac{3}{5} - \frac{4}{5}i
            \]

            \item [c.)] We have that
            \[
                \parens{\frac{2 + i}{3 - 2i}}^2 =
                \frac{2 + i}{3 - 2i} \cdot \frac{2 + i}{3 - 2i} =
                \frac{3 + 4i}{5 - 12i} = 
                \frac{3 + 4i}{5 - 12i} \cdot \frac{5 + 12i}{5 + 12i} =
                \frac{-33 + 56i}{169}
            \]
            \[ = -\frac{33}{169} + \frac{56}{169}i \]

            \item [d.)] Awd
        \end{itemize}
    \end{itemize}
\end{document}